WIP

src/Weakest.v
@@ -1431,60 +1431,65 @@ Section FAIR.
   .
   Admitted.
 
-  Definition Eventually (k: nat) (P: iProp): iProp :=
-    □ PosEx k ** (Ongoing k ∨ ((□ Done k) ** P)).
+  Definition Eventually (k: nat) (P: iProp) (Q: iProp): iProp :=
+    □ PosEx k ** ((Ongoing k ** P) ∨ ((□ Done k) ** Q)).
 
-  Lemma pending_eventually P k
+  Lemma pending_eventually P Q k
     :
     (Pending k)
       -∗
-      (#=> Eventually k P).
-  Proof.
-  Admitted.
-
-  Lemma eventually_done k P
-    :
-    (Done k)
-      -∗
-      (Eventually k P)
-      -∗
-      (P ** (P -* Eventually k P)).
-  Proof.
-  Admitted.
-
-  Lemma eventually_intro_ongoing k P
-    :
-    (Ongoing k)
-      -∗
-      (Eventually k P).
-  Proof.
-  Admitted.
-
-  Lemma eventually_intro_done k P
-    :
-    (Done k)
-      -∗
       P
       -∗
-      (Eventually k P).
+      (#=> Eventually k P Q).
   Proof.
   Admitted.
 
-  Lemma eventually_finish k P
+  Lemma eventually_done k P Q
     :
-    (Eventually k P)
+    (Done k)
       -∗
-      ((□ Done k) ∨ (Ongoing k ** (Done k -* P -* Eventually k P))).
+      (Eventually k P Q)
+      -∗
+      (Q ** (Q -* Eventually k P Q)).
   Proof.
   Admitted.
 
-  Lemma eventually_obligation k P
+  Lemma eventually_intro_done k P Q
     :
-    (Eventually k P)
+    (Done k)
+      -∗
+      Q
+      -∗
+      (Eventually k P Q).
+  Proof.
+  Admitted.
+
+  Lemma eventually_finish k P Q
+    :
+    (Eventually k P Q)
+      -∗
+      ((□ Done k) ∨ (Ongoing k ** P ** (Done k -* Q -* Eventually k P Q))).
+  Proof.
+  Admitted.
+
+  Lemma eventually_unfold k P Q
+    :
+    (Eventually k P Q)
+      -∗
+      ((Ongoing k ** P ** (Done k -* Q -* Eventually k P Q) ∧ (Ongoing k -* P -* Eventually k P Q)) ∨
+         (Done k ** Q ** (Q -* Eventually k P Q))).
+  Proof.
+  Admitted.
+
+  Lemma eventually_obligation k P Q
+    :
+    (Eventually k P Q)
       -∗
       (Ready k).
   Proof.
   Admitted.
+
+  Global Opaque Eventually.
 
   Variable state_tgt: Type.
   Definition St_tgt: state_tgt -> iProp. Admitted.
@@ -1870,16 +1875,22 @@ Section FAIR.
   Proof.
   Admitted.
 
+
   Context `{SRCORD: @GRA.inG (@FairRA.t ident_src Ord.t _) Σ}.
   Context `{TGTORD: @GRA.inG (@FairRA.t ident_tgt nat _) Σ}.
+  Context `{IDENTSRC: @GRA.inG (identSrcRA ident_src wf_src) Σ}.
+  Context `{IDENTTGT: @GRA.inG (identTgtRA ident_tgt) Σ}.
 
-  Lemma fsim_fairL o f r g R_src R_tgt
+
+
+  Lemma fsim_fairL f r g R_src R_tgt
         (Q: R_src -> R_tgt -> list nat -> iProp)
-        os ktr_src itr_tgt
+        os ktr_src itr_tgt im_src0
     :
-    (Infsum (fun i: sig (fun i => f i = Flag.fail) => FairRA.white (proj1_sig i) (Ord.from_nat 1)))
+    (OwnM (Auth.white (Excl.just im_src0: @Excl.t _): identSrcRA ident_src wf_src))
       -∗
-      ((Infsum (fun i: sig (fun i => f i = Flag.success) => FairRA.white (proj1_sig i) o)) -* (fsim r g Q (ktr_src tt) itr_tgt os))
+      (∃ im_src1, ⌜fair_update im_src0 im_src1 f⌝ ∧
+                    ((OwnM (Auth.white (Excl.just im_src1: @Excl.t _): identSrcRA ident_src wf_src)) -∗ (fsim r g Q (ktr_src tt) itr_tgt os)))
       -∗
       (fsim r g Q (trigger (Fair f) >>= ktr_src) itr_tgt os).
   Proof.
@@ -1887,15 +1898,41 @@ Section FAIR.
 
   Lemma fsim_fairR f r g R_src R_tgt
         (Q: R_src -> R_tgt -> list nat -> iProp)
-        os itr_src ktr_tgt
+        os itr_src ktr_tgt im_tgt0
     :
-    (Infsum (fun i: sig (fun i => f i = Flag.success) => (∃ a, FairRA.black (proj1_sig i) a)%I))
+    (OwnM (Auth.white (Excl.just im_tgt0: @Excl.t _): identTgtRA ident_tgt))
       -∗
-      ((Infsum (fun i: sig (fun i => f i = Flag.fail) => FairRA.white (proj1_sig i) 1)) -* (fsim r g Q itr_src (ktr_tgt tt) os))
+      (∀ im_tgt1, ⌜fair_update im_tgt0 im_tgt1 f⌝ -* (OwnM (Auth.white (Excl.just im_tgt1: @Excl.t _): identTgtRA ident_tgt)) -* fsim r g Q itr_src (ktr_tgt tt) os)
       -∗
-      (fsim r g Q itr_src (trigger (Fair f) >>= ktr_tgt) os).
+      (fsim r g Q itr_src (trigger (Fair f) >>= ktr_tgt) os)
+  .
   Proof.
   Admitted.
+
+  (* Lemma fsim_fairL o f r g R_src R_tgt *)
+  (*       (Q: R_src -> R_tgt -> list nat -> iProp) *)
+  (*       os ktr_src itr_tgt *)
+  (*   : *)
+  (*   (Infsum (fun i: sig (fun i => f i = Flag.fail) => FairRA.white (proj1_sig i) (Ord.from_nat 1))) *)
+  (*     -∗ *)
+  (*     ((Infsum (fun i: sig (fun i => f i = Flag.success) => FairRA.white (proj1_sig i) o)) -* (fsim r g Q (ktr_src tt) itr_tgt os)) *)
+  (*     -∗ *)
+  (*     (fsim r g Q (trigger (Fair f) >>= ktr_src) itr_tgt os). *)
+  (* Proof. *)
+  (* Admitted. *)
+
+  (* Lemma fsim_fairR f r g R_src R_tgt *)
+  (*       (Q: R_src -> R_tgt -> list nat -> iProp) *)
+  (*       os itr_src ktr_tgt *)
+  (*   : *)
+  (*   (Infsum (fun i: sig (fun i => f i = Flag.success) => (∃ a, FairRA.black (proj1_sig i) a)%I)) *)
+  (*     -∗ *)
+  (*     ((Infsum (fun i: sig (fun i => f i = Flag.fail) => FairRA.white (proj1_sig i) 1)) -* (fsim r g Q itr_src (ktr_tgt tt) os)) *)
+  (*     -∗ *)
+  (*     (fsim r g Q itr_src (trigger (Fair f) >>= ktr_tgt) os). *)
+  (* Proof. *)
+  (* Admitted. *)
+
 End FAIR.
 
 From Fairness Require Export Red IRed.
